SStructTT/SStruct/Erasure/Syntax.lean
@@ -4,19 +4,16 @@ import SStructTT.SStruct.Dynamic.Typed
 namespace SStruct.Erasure
 variable (Srt : Type)
 
-inductive Ctrl where
-  | keep
-  | drop
-
 inductive Tm where
   | var  (x : Var)
-  | lam  (m : Tm) (c : Ctrl) (s : Srt)
+  | lam  (m : Tm) (s : Srt)
   | app  (m n : Tm)
   | tup  (m n : Tm) (s : Srt)
-  | prj (m n : Tm) (c1 c2 : Ctrl)
+  | prj  (m n : Tm)
   | tt | ff
   | ite  (m n1 n2 : Tm)
   | rw   (m : Tm)
+  | drop (ms : List Tm) (m : Tm)
   | ptr  (l : Nat)
   | null
 
@@ -30,14 +27,15 @@ instance : Ids (Tm Srt) where
 def rename_rec (ξ : Var -> Var) (m : Tm Srt) : Tm Srt :=
   match m with
   | var x => var (ξ x)
-  | lam m c s => lam (rename_rec (upren ξ) m) c s
+  | lam m s => lam (rename_rec (upren ξ) m) s
   | app m n => app (rename_rec ξ m) (rename_rec ξ n)
   | tup m n s => tup (rename_rec ξ m) (rename_rec ξ n) s
-  | prj m n c1 c2 => prj (rename_rec ξ m) (rename_rec (upren $ upren ξ) n) c1 c2
+  | prj m n => prj (rename_rec ξ m) (rename_rec (upren $ upren ξ) n)
   | tt => tt
   | ff => ff
   | ite m n1 n2 => ite (rename_rec ξ m) (rename_rec ξ n1) (rename_rec ξ n2)
   | rw m => rw (rename_rec ξ m)
+  | drop ms m => drop (ms.map (rename_rec ξ)) (rename_rec ξ m)
   | ptr l => ptr l
   | null => null
 
@@ -45,53 +43,56 @@ instance : Rename (Tm Srt) where
   rename := rename_rec
 
 namespace Rename
-variable (ξ : Var -> Var) (A B m n n1 n2 : Tm Srt) (x i l : Nat) (c c1 c2 : Ctrl) (s : Srt)
+variable (ξ : Var -> Var) (A B m n n1 n2 : Tm Srt) (ms : List (Tm Srt)) (x i l : Nat) (s : Srt)
 
-@[asimp]lemma ids  : rename ξ (ids x) = @ids (Tm Srt) _ (ξ x) := by rfl
-@[asimp]lemma lam  : rename ξ (lam m c s) = lam (rename (upren ξ) m) c s := by rfl
-@[asimp]lemma app  : rename ξ (app m n) = app (rename ξ m) (rename ξ n) := by rfl
-@[asimp]lemma tup  : rename ξ (tup m n s) = tup (rename ξ m) (rename ξ n) s := by rfl
-@[asimp]lemma prj  : rename ξ (prj m n c1 c2) = prj (rename ξ m) (rename (upren $ upren ξ) n) c1 c2 := by rfl
-@[asimp]lemma tt   : rename ξ (@tt Srt) = tt := by rfl
-@[asimp]lemma ff   : rename ξ (@ff Srt) = ff := by rfl
-@[asimp]lemma ite  : rename ξ (ite m n1 n2) = ite (rename ξ m) (rename ξ n1) (rename ξ n2) := by rfl
-@[asimp]lemma ptr  : rename ξ (@ptr Srt l) = ptr l := by rfl
-@[asimp]lemma rw   : rename ξ (rw m) = rw (rename ξ m) := by rfl
-@[asimp]lemma null : rename ξ (@null Srt) = null := by rfl
+@[asimp]lemma ids  : rename ξ (ids x) = @ids (Tm Srt) _ (ξ x) := by apply rename_rec.eq_def
+@[asimp]lemma lam  : rename ξ (lam m s) = lam (rename (upren ξ) m) s := by apply rename_rec.eq_def
+@[asimp]lemma app  : rename ξ (app m n) = app (rename ξ m) (rename ξ n) := by apply rename_rec.eq_def
+@[asimp]lemma tup  : rename ξ (tup m n s) = tup (rename ξ m) (rename ξ n) s := by apply rename_rec.eq_def
+@[asimp]lemma prj  : rename ξ (prj m n) = prj (rename ξ m) (rename (upren $ upren ξ) n) := by apply rename_rec.eq_def
+@[asimp]lemma tt   : rename ξ (@tt Srt) = tt := by apply rename_rec.eq_def
+@[asimp]lemma ff   : rename ξ (@ff Srt) = ff := by apply rename_rec.eq_def
+@[asimp]lemma ite  : rename ξ (ite m n1 n2) = ite (rename ξ m) (rename ξ n1) (rename ξ n2) := by apply rename_rec.eq_def
+@[asimp]lemma rw   : rename ξ (rw m) = rw (rename ξ m) := by apply rename_rec.eq_def
+@[asimp]lemma drop : rename ξ (drop ms m) = drop (ms.map (rename ξ)) (rename ξ m) := by apply rename_rec.eq_def
+@[asimp]lemma ptr  : rename ξ (@ptr Srt l) = ptr l := by apply rename_rec.eq_def
+@[asimp]lemma null : rename ξ (@null Srt) = null := by apply rename_rec.eq_def
 @[asimp]lemma rename_rec : rename_rec ξ m = rename ξ m := by rfl
 end Rename
 
 def subst_rec (σ : Var -> Tm Srt) (m : Tm Srt) : Tm Srt :=
   match m with
   | var x => σ x
-  | lam m c s => lam (subst_rec (up σ) m) c s
+  | lam m s => lam (subst_rec (up σ) m) s
   | app m n => app (subst_rec σ m) (subst_rec σ n)
   | tup m n s => tup (subst_rec σ m) (subst_rec σ n) s
-  | prj m n c1 c2 => prj (subst_rec σ m) (subst_rec (upn 2 σ) n) c1 c2
+  | prj m n => prj (subst_rec σ m) (subst_rec (upn 2 σ) n)
   | tt => tt
   | ff => ff
   | ite m n1 n2 => ite (subst_rec σ m) (subst_rec σ n1) (subst_rec σ n2)
   | rw m => rw (subst_rec σ m)
   | ptr l => ptr l
+  | drop ms m => drop (ms.map (subst_rec σ)) (subst_rec σ m)
   | null => null
 
 instance : Subst (Tm Srt) where
   subst := subst_rec
 
 namespace Subst
-variable (σ : Var -> Tm Srt) (A B m n n1 n2 : Tm Srt) (x i l : Nat) (c c1 c2 : Ctrl) (s : Srt)
+variable (σ : Var -> Tm Srt) (A B m n n1 n2 : Tm Srt) (ms : List (Tm Srt)) (x i l : Nat) (s : Srt)
 
-@[asimp]lemma ids  : subst σ (ids x) = σ x := by rfl
-@[asimp]lemma lam  : subst σ (lam m c s) = lam (subst (up σ) m) c s := by rfl
-@[asimp]lemma app  : subst σ (app m n) = app (subst σ m) (subst σ n) := by rfl
-@[asimp]lemma tup  : subst σ (tup m n s) = tup (subst σ m) (subst σ n) s := by rfl
-@[asimp]lemma prj  : subst σ (prj m n c1 c2) = prj (subst σ m) (subst (upn 2 σ) n) c1 c2 := by rfl
-@[asimp]lemma tt   : subst σ (@tt Srt) = tt := by rfl
-@[asimp]lemma ff   : subst σ (@ff Srt) = ff := by rfl
-@[asimp]lemma ite  : subst σ (ite m n1 n2) = ite (subst σ m) (subst σ n1) (subst σ n2) := by rfl
-@[asimp]lemma rw   : subst σ (rw m) = rw (subst σ m) := by rfl
-@[asimp]lemma ptr  : subst σ (@ptr Srt l) = ptr l := by rfl
-@[asimp]lemma null : subst σ (@null Srt) = null := by rfl
+@[asimp]lemma ids  : subst σ (ids x) = σ x := by apply subst_rec.eq_def
+@[asimp]lemma lam  : subst σ (lam m s) = lam (subst (up σ) m) s := by apply subst_rec.eq_def
+@[asimp]lemma app  : subst σ (app m n) = app (subst σ m) (subst σ n) := by apply subst_rec.eq_def
+@[asimp]lemma tup  : subst σ (tup m n s) = tup (subst σ m) (subst σ n) s := by apply subst_rec.eq_def
+@[asimp]lemma prj  : subst σ (prj m n) = prj (subst σ m) (subst (upn 2 σ) n) := by apply subst_rec.eq_def
+@[asimp]lemma tt   : subst σ (@tt Srt) = tt := by apply subst_rec.eq_def
+@[asimp]lemma ff   : subst σ (@ff Srt) = ff := by apply subst_rec.eq_def
+@[asimp]lemma ite  : subst σ (ite m n1 n2) = ite (subst σ m) (subst σ n1) (subst σ n2) := by apply subst_rec.eq_def
+@[asimp]lemma rw   : subst σ (rw m) = rw (subst σ m) := by apply subst_rec.eq_def
+@[asimp]lemma drop : subst σ (drop ms m) = drop (ms.map (subst σ)) (subst σ m) := by apply subst_rec.eq_def
+@[asimp]lemma ptr  : subst σ (@ptr Srt l) = ptr l := by apply subst_rec.eq_def
+@[asimp]lemma null : subst σ (@null Srt) = null := by apply subst_rec.eq_def
 @[asimp]lemma subst_rec : subst_rec σ m = subst σ m := by rfl
 end Subst
 
@@ -101,18 +102,23 @@ lemma up_upren (ξ : Var -> Var) :
   funext x; cases x <;> asimp
 
 lemma rename_subst ξ (m : Tm Srt) : rename ξ m = m.[ren ξ] := by
-  induction m generalizing ξ with
+  induction m using
+    Tm.rec (motive_2 := fun ms => ∀ξ, ms.map (rename ξ) = ms.map (. .[ren ξ]))
+  generalizing ξ with
   | var => asimp
-  | lam m c s ihm => asimp[up_upren, ihm]
+  | lam m s ihm => asimp[up_upren, ihm]
   | app m n ihm ihn => asimp[ihm, ihn]
   | tup m n s ihm ihn => asimp[ihm, ihn]
-  | prj m n c1 c2 ihm ihn => asimp[up_upren, ihm, ihn]
+  | prj m n ihm ihn => asimp[up_upren, ihm, ihn]
   | tt => asimp
   | ff => asimp
   | ite m n1 n2 ihm ihn1 ihn2 => asimp[up_upren, ihm, ihn1, ihn2]
   | rw m ihm => asimp[ihm]
+  | drop ms m ihms ihm => asimp[up_upren, ihms, ihm]
   | ptr l => asimp
   | null => asimp
+  | nil ξ => simp
+  | cons ξ => simp; aesop
 
 lemma up_ids : up ids = @ids (Tm Srt) _ := by
   funext x
@@ -121,18 +127,23 @@ lemma up_ids : up ids = @ids (Tm Srt) _ := by
   | succ => asimp
 
 lemma subst_id (m : Tm Srt) : m.[ids] = m := by
-  induction m with
+  induction m using
+    Tm.rec (motive_2 := fun ms => ms.map (. .[ids]) = ms)
+  with
   | var => asimp
-  | lam m c s ihm => asimp[up_ids, ihm]
+  | lam m s ihm => asimp[up_ids, ihm]
   | app m n ihm ihn => asimp[ihm, ihn]
   | tup m n s ihm ihn => asimp[ihm, ihn]
-  | prj m n c1 c2 ihm ihn => asimp[up_ids, ihm, ihn]
+  | prj m n ihm ihn => asimp[up_ids, ihm, ihn]
   | tt => asimp
   | ff => asimp
   | ite m n1 n2 ihm ihn1 ihn2 => asimp[up_ids, ihm, ihn1, ihn2]
   | rw m ihm => asimp[ihm]
+  | drop ms m ihms ihm => asimp[ihms, ihm]
   | ptr l => asimp
   | null => asimp
+  | nil => simp
+  | cons => simp; aesop
 
 lemma up_comp_upren (ξ : Var -> Var) (σ : Var -> Tm Srt) :
     up (ξ !>> σ) = upren ξ !>> up σ := by
@@ -142,18 +153,23 @@ lemma up_comp_upren (ξ : Var -> Var) (σ : Var -> Tm Srt) :
   | succ => asimp
 
 lemma ren_subst_comp ξ σ (m : Tm Srt) : m.[ren ξ].[σ] = m.[ξ !>> σ] := by
-  induction m generalizing ξ σ with
+  induction m using
+    Tm.rec (motive_2 := fun ms => ∀ξ σ, (ms.map (. .[ren ξ])).map (. .[σ]) = ms.map (. .[ξ !>> σ]))
+  generalizing ξ σ with
   | var => asimp
-  | lam m c s ihm => asimp[up_upren, up_comp_upren, ihm]
+  | lam m c ihm => asimp[up_upren, up_comp_upren, ihm]
   | app m n ihm ihn => asimp[ihm, ihn]
   | tup m n s ihm ihn => asimp[ihm, ihn]
-  | prj m n c1 c2 ihm ihn => asimp[up_upren, up_comp_upren, ihm, ihn]
+  | prj m n ihm ihn => asimp[up_upren, up_comp_upren, ihm, ihn]
   | tt => asimp
   | ff => asimp
   | ite m n1 n2 ihm ihn1 ihn2 => asimp[up_upren, up_comp_upren, ihm, ihn1, ihn2]
   | rw m ihm => asimp[ihm]
+  | drop ms m ihms ihm => asimp[ihms, ihm]
   | ptr l => asimp
   | null => asimp
+  | nil => simp
+  | cons => simp; aesop
 
 lemma up_comp_ren (σ : Var -> Tm Srt) (ξ : Var -> Var) :
     up σ !>> rename (upren ξ) = up (σ !>> rename ξ)  := by
@@ -167,18 +183,23 @@ lemma up_comp_ren (σ : Var -> Tm Srt) (ξ : Var -> Var) :
     rw[h1, h2]; rfl
 
 lemma subst_ren_comp σ ξ (m : Tm Srt) : m.[σ].[ren ξ] = m.[σ !>> rename ξ] := by
-  induction m generalizing σ ξ with
+  induction m using
+    Tm.rec (motive_2 := fun ms => ∀ξ σ, (ms.map (. .[σ])).map (. .[ren ξ]) = ms.map (. .[σ !>> rename ξ]))
+  generalizing σ ξ with
   | var => asimp[rename_subst]
-  | lam m c s ihm => asimp[up_upren, up_comp_ren, ihm]
+  | lam m s ihm => asimp[up_upren, up_comp_ren, ihm]
   | app m n ihm ihn => asimp[ihm, ihn]
   | tup m n s ihm ihn => asimp[ihm, ihn]
-  | prj m n c1 c2 ihm ihn => asimp[up_upren, up_comp_ren, ihm, ihn]
+  | prj m n ihm ihn => asimp[up_upren, up_comp_ren, ihm, ihn]
   | tt => asimp
   | ff => asimp
   | ite m n1 n2 ihm ihn1 ihn2 => asimp[up_upren, up_comp_ren, ihm, ihn1, ihn2]
   | rw m ihm => asimp[ihm]
+  | drop ms m ihms ihm => asimp[ihms, ihm]
   | ptr l => asimp
   | null => asimp
+  | nil => simp
+  | cons => simp; aesop
 
 lemma up_comp (σ τ : Var -> Tm Srt) :  up σ !> up τ = up (σ !> τ) := by
   funext x
@@ -192,18 +213,23 @@ lemma up_comp (σ τ : Var -> Tm Srt) :  up σ !> up τ = up (σ !> τ) := by
     rfl
 
 lemma subst_comp (σ τ : Var -> Tm Srt) m : m.[σ].[τ] = m.[σ !> τ] := by
-  induction m generalizing σ τ with
+  induction m using
+    Tm.rec (motive_2 := fun ms => ∀σ τ, (ms.map (. .[σ])).map (. .[τ]) = ms.map (. .[σ !> τ]))
+  generalizing σ τ with
   | var => asimp
-  | lam m c s ihm => asimp[up_comp, ihm]
+  | lam m s ihm => asimp[up_comp, ihm]
   | app m n ihm ihn => asimp[ihm, ihn]
   | tup m n s ihm ihn => asimp[ihm, ihn]
-  | prj m n c1 c2 ihm ihn => asimp[up_comp, ihm, ihn]
+  | prj m n ihm ihn => asimp[up_comp, ihm, ihn]
   | tt => asimp
   | ff => asimp
   | ite m n1 n2 ihm ihn1 ihn2 => asimp[up_comp, ihm, ihn1, ihn2]
   | rw m ihm => asimp[ihm]
+  | drop ms m ihms ihm => asimp[ihms, ihm]
   | ptr l => asimp
   | null => asimp
+  | nil => simp
+  | cons => simp; aesop
 
 instance : SubstLemmas (Tm Srt) where
   rename_subst := rename_subst
