SStructTT/SStruct/Dynamic/Inversion.lean
@@ -22,10 +22,16 @@ lemma Typed.lam_im_inv' {Γ} {Δ : Ctx Srt} {A T m s} :
   case lam_im B _ _ sA _ _ _ _ _ =>
     cases e; exists B, sA; aesop
   case lam_ex => cases e
+  case weak wk _ ih =>
+    have ⟨B, sA, tym, eq2⟩ := ih e
+    exists B, sA; and_intros
+    . apply Typed.weak
+      constructor; assumption
+      assumption
+    . assumption
   case conv eq1 _ _ ih =>
     have ⟨B, sA, tym, eq2⟩ := ih e
-    exists B, sA
-    and_intros
+    exists B, sA; and_intros
     . assumption
     . apply Conv.trans
       apply Conv.sym eq1
@@ -33,21 +39,25 @@ lemma Typed.lam_im_inv' {Γ} {Δ : Ctx Srt} {A T m s} :
 
 lemma Typed.lam_ex_inv' {Γ} {Δ : Ctx Srt} {A T m s} :
     Γ ;; Δ ⊢ .lam A m .ex s : T ->
-    ∃ B rA sA,
-      RSrt rA sA ∧
-      A :: Γ ;; A :⟨rA, sA⟩ Δ ⊢ m : B ∧
+    ∃ B sA,
+      A :: Γ ;; A :⟨.ex, sA⟩ Δ ⊢ m : B ∧
       T === .pi A B .ex s := by
   generalize e: Tm.lam A m .ex s = x
   intro ty; induction ty generalizing A m s
   all_goals try trivial
   case lam_im => cases e
-  case lam_ex B _ rA _ sA _ rs _ _ _ _ =>
-    cases e; exists B, rA, sA; aesop
-  case conv eq1 _ _ ih =>
-    have ⟨B, sA, rA, rs, tym, eq2⟩ := ih e
-    exists B, sA, rA
-    and_intros
+  case lam_ex B _ _ sA _ _ _ _ _ =>
+    cases e; exists B, sA; aesop
+  case weak wk _ ih =>
+    have ⟨B, sA, tym, eq2⟩ := ih e
+    exists B, sA; and_intros
+    . apply Typed.weak
+      constructor; assumption
+      assumption
     . assumption
+  case conv eq1 _ _ ih =>
+    have ⟨B, sA, tym, eq2⟩ := ih e
+    exists B, sA; and_intros
     . assumption
     . apply Conv.trans
       apply Conv.sym eq1
@@ -65,15 +75,84 @@ lemma Typed.tup_im_inv' {Γ} {Δ : Ctx Srt} {T m n s} :
   case tup_im A B _ _ _ _ _ _ _ _ =>
     cases e; exists A, B; aesop
   case tup_ex => cases e
+  case weak wk _ ih =>
+    have ⟨A, B, _, _, eq2⟩ := ih e
+    exists A, B; and_intros
+    . apply Typed.weak
+      assumption
+      assumption
+    . assumption
+    . assumption
   case conv eq1 _ _ ih =>
     have ⟨A, B, _, _, eq2⟩ := ih e
-    exists A, B
-    and_intros
+    exists A, B; and_intros
     . assumption
     . assumption
     . apply Conv.trans
       apply Conv.sym eq1
       apply eq2
+
+lemma Merge.split_weaken {Δ1 Δ2 Δ3 Δ3' : Ctx Srt} :
+    Merge Δ1 Δ2 Δ3 -> Weaken Δ3 Δ3' ->
+    ∃ Δ1' Δ2', Merge Δ1' Δ2' Δ3' ∧ Weaken Δ1 Δ1' ∧ Weaken Δ2 Δ2' := by
+  intro mrg wk; induction mrg generalizing Δ3'
+  case nil => cases wk; exists [], []; aesop
+  case contra A s h mrg ih =>
+    cases wk
+    case cons Δw wk =>
+      have ⟨Δ1', Δ2', mrg', wk1, wk2⟩ := ih wk
+      exists A :⟨.ex, s⟩ Δ1', A :⟨.ex, s⟩ Δ2'; and_intros
+      . constructor <;> assumption
+      . constructor; assumption
+      . constructor; assumption
+    case weak Δw h wk =>
+      have ⟨Δ1', Δ2', mrg', wk1, wk2⟩ := ih wk
+      exists A :⟨.ex, s⟩ Δ1', A :⟨.ex, s⟩ Δ2'; and_intros
+      . constructor <;> assumption
+      . constructor; assumption
+      . constructor; assumption
+  case left A s mrg ih =>
+    cases wk
+    case cons Δw wk =>
+      have ⟨Δ1', Δ2', mrg', wk1, wk2⟩ := ih wk
+      exists A :⟨.ex, s⟩ Δ1', A :⟨.im, s⟩ Δ2'; and_intros
+      . constructor; assumption
+      . constructor; assumption
+      . constructor; assumption
+    case weak Δw h wk =>
+      have ⟨Δ1', Δ2', mrg', wk1, wk2⟩ := ih wk
+      exists A :⟨.ex, s⟩ Δ1', A :⟨.im, s⟩ Δ2'; and_intros
+      . constructor; assumption
+      . constructor; assumption
+      . constructor; assumption
+  case right A s mrg ih =>
+    cases wk
+    case cons Δw wk =>
+      have ⟨Δ1', Δ2', mrg', wk1, wk2⟩ := ih wk
+      exists A :⟨.im, s⟩ Δ1', A :⟨.ex, s⟩ Δ2'; and_intros
+      . constructor; assumption
+      . constructor; assumption
+      . constructor; assumption
+    case weak Δw h wk =>
+      have ⟨Δ1', Δ2', mrg', wk1, wk2⟩ := ih wk
+      exists A :⟨.im, s⟩ Δ1', A :⟨.ex, s⟩ Δ2'; and_intros
+      . constructor; assumption
+      . constructor; assumption
+      . constructor; assumption
+  case im A s mrg ih =>
+    cases wk
+    case cons Δw wk =>
+      have ⟨Δ1', Δ2', mrg', wk1, wk2⟩ := ih wk
+      exists A :⟨.im, s⟩ Δ1', A :⟨.im, s⟩ Δ2'; and_intros
+      . constructor; assumption
+      . constructor; assumption
+      . constructor; assumption
+    case weak Δw h wk =>
+      have ⟨Δ1', Δ2', mrg', wk1, wk2⟩ := ih wk
+      exists A :⟨.im, s⟩ Δ1', A :⟨.ex, s⟩ Δ2'; and_intros
+      . constructor; assumption
+      . constructor; assumption
+      . constructor <;> assumption
 
 lemma Typed.tup_ex_inv' {Γ} {Δ : Ctx Srt} {T m n s} :
     Γ ;; Δ ⊢ .tup m n .ex s : T ->
@@ -88,10 +167,19 @@ lemma Typed.tup_ex_inv' {Γ} {Δ : Ctx Srt} {T m n s} :
   case tup_im => cases e
   case tup_ex Δ1 Δ2 Δ A B _ _ _ _ _ _ _ _ _ _ =>
     cases e; exists Δ1, Δ2, A, B; aesop
+  case weak wk _ ih =>
+    have ⟨Δ1, Δ2, A, B, mrg, tym, tyn, eq2⟩ := ih e
+    have ⟨Δ1', Δ2', mrg', wk1, wk2⟩ := mrg.split_weaken wk
+    exists Δ1', Δ2', A, B; and_intros
+    . assumption
+    . apply Typed.weak wk1
+      assumption
+    . apply Typed.weak wk2
+      assumption
+    . assumption
   case conv eq1 _ _ ih =>
     have ⟨Δ1, Δ2, A, B, mrg, _, _, eq2⟩ := ih e
-    exists Δ1, Δ2, A, B
-    and_intros
+    exists Δ1, Δ2, A, B; and_intros
     . assumption
     . assumption
     . assumption
@@ -120,9 +208,9 @@ lemma Typed.lam_im_inv {Γ} {Δ : Ctx Srt} {A A' B m s s'} :
 
 lemma Typed.lam_ex_inv {Γ} {Δ : Ctx Srt} {A A' B m s s'} :
     Γ ;; Δ ⊢ .lam A m .ex s : .pi A' B .ex s' ->
-    ∃ rA sA, RSrt rA sA ∧ A' :: Γ ;; A' :⟨rA, sA⟩ Δ ⊢ m : B := by
+    ∃ sA, A' :: Γ ;; A' :⟨.ex, sA⟩ Δ ⊢ m : B := by
   intro ty
-  have ⟨B, rA, sA, rs, tym, eq⟩ := ty.lam_ex_inv'
+  have ⟨B, sA, tym, eq⟩ := ty.lam_ex_inv'
   have ⟨_, _, eqA, eqB⟩ := Static.Conv.pi_inj eq
   have ⟨s, i, tyP⟩ := ty.toStatic.validity
   have ⟨_, _, _, tyB, _⟩ := tyP.pi_inv
@@ -132,12 +220,10 @@ lemma Typed.lam_ex_inv {Γ} {Δ : Ctx Srt} {A A' B m s s'} :
   have ty1 := tyA'.preservation' rd'
   have ty2 := tyA.preservation' rd
   have e := Static.Typed.unique ty1 ty2
-  subst_vars; exists rA, sA'
+  subst_vars; exists sA'
   replace tyB := Static.Typed.conv_ctx eqA.sym tyA tyB
-  and_intros
-  . assumption
-  . apply Typed.conv_ctx eqA tyA'
-    apply Typed.conv eqB.sym tym tyB
+  apply Typed.conv_ctx eqA tyA'
+  apply Typed.conv eqB.sym tym tyB
 
 lemma Typed.tup_im_inv {Γ} {Δ : Ctx Srt} {A B m n s s'} :
     Γ ;; Δ ⊢ .tup m n .im s : .sig A B .im s' ->
